case_studies/lin_lam/tenv.v
@@ -1,0 +1,40 @@
+(** Common type enviroments abbreviations for llc
+
+. note: needs constants for purely_linear. Shoud be abstracted better
+ *)
+
+Require Import ARS core fintype stlc.
+Import ScopedNotations.
+From Coq Require Import Unicode.Utf8.
+From Coq Require Import Logic.FunctionalExtensionality.
+
+(* Separation logic / CARVe imports *)
+Require Import VST.msl.sepalg.
+Require Import VST.msl.functors.
+From CARVe.contexts Require Import total_fun.
+ From CARVe.algebras Require Import purely_linear. 
+
+(* General settings *)
+Set Implicit Arguments.
+
+(* This should be in fintype, but it's not  *)
+
+Lemma fin_eq {n} (x y : fin n) : {x = y} + {x <> y}.
+Proof. induction n; [destruct x | decide equality]. Qed.
+
+(** An EqDec instance for fin n *)
+
+#[global] Program Instance EqDec_fin (n : nat) : EqDec (fin n) :=
+  {| eq_dec := @fin_eq n |}.
+
+Definition tenv n := tfctx (fin n) ty mult.
+
+Definition emptyT := empty_tfctx (fin 0) _ _ (Unit, zero).
+
+(* can this go in total_fun ? How? *)
+Property join_emptyT: forall Δ₁ Δ₂, join Δ₁ Δ₂ emptyT → Δ₁ = emptyT ∧ Δ₂ = emptyT.
+Proof.
+  split; apply functional_extensionality; intro x; contradiction.
+Qed.
+
+(* put here other properties of interest not linked to a specific type system*)
