case_studies/lin_lam/typing.v
@@ -1,0 +1,94 @@
+(* ======================================================= *)
+(* Typing and progress for pure llc      *)
+(* (contexts as total maps)                                *)
+(* ======================================================= *)
+
+
+Require Import ARS core fintype stlc step tenv.
+Import ScopedNotations.
+From Coq Require Import Unicode.Utf8.
+From Coq Require Import Lia.
+From Hammer Require Import Tactics.
+From Coq Require Import Logic.FunctionalExtensionality.
+
+(* Separation logic / CARVe imports *)
+Require Import VST.msl.sepalg.
+Require Import VST.msl.functors.
+From CARVe.contexts Require Import total_fun.
+From CARVe.algebras Require Import purely_linear.
+
+(* General settings *)
+Set Implicit Arguments.
+
+(* ----------------------------------- *)
+(* Typing judgment                     *)
+(* ----------------------------------- *)
+
+Inductive has_type {n} (Δ : tenv n) : tm n → ty → Prop :=
+
+| t_Var :
+  forall (T : ty) (fn : fin n),
+    lookup_tfctx _ _ _ Δ fn = (T, one) ->
+    exh _ _  _ hal
+                  (update_tfctx
+                     _ _
+                     _ Δ fn T
+                     zero) ->
+    has_type Δ (var_tm fn) T
+
+| t_Abs :
+  forall (T1 T2 : ty) e1,
+    has_type (scons (T2, one) Δ) e1 T1 →
+    has_type Δ (lam T2 e1) (Fun T2 T1)
+
+| t_App :
+  forall (Δ1 Δ2 : tenv n) (T1 T2 : ty) (e1 e2 : tm n),
+    has_type Δ1 e1 (Fun T2 T1) →
+    has_type Δ2 e2 T2 →
+    join Δ1 Δ2 Δ →
+    has_type Δ (Core.app e1 e2) T1.
+
+Notation "Δ '|-' e ':' T" := (has_type Δ e T) (at level 40).
+
+(* If Δ₁ ⋈ Δ₂ = Δ, then types must match at each input x *)
+Lemma join_types_match :
+  forall {n} {Δ Δ1 Δ2 : tenv n} (x : fin n),
+    join Δ1 Δ2 Δ →
+    fst (Δ x) = fst (Δ1 x) ∧ fst (Δ x) = fst (Δ2 x).
+Proof.
+  intros n Δ Δ1 Δ2 x Hjoin.
+  specialize (Hjoin x).
+  destruct (Δ1 x) as [t1 m1].
+  destruct (Δ2 x) as [t2 m2].
+  destruct (Δ x) as [t m].
+  (* From the definition of join, t = t1 and t = t2 *)
+  cbn. sauto q: on.
+Qed.
+
+
+(* ------------------------------------- *)
+(* Canonical forms lemma                 *)
+(* ------------------------------------- *)
+
+Lemma canonical_forms_fun : forall (M : tm 0) T1 T2,
+  has_type emptyT M (Fun T1 T2) →
+  value M →
+  exists N U, M = (lam U N).
+Proof. sauto lq: on . Qed.    
+
+(* Progress *)
+Lemma progress (M : tm 0) : forall T,
+  has_type emptyT M T → value M ∨ exists M', step M M'.  
+Proof.
+  dependent induction M; intros; try sfirstorder.
+  - (* app case *)
+    right. inversion H; subst.
+    apply join_emptyT in H5; sintuition.
+    destruct (IHM1 M1 eq_refl JMeq_refl (Fun T2  T) H2).
+    + (* t1 is a value *)
+      apply canonical_forms_fun in H2; [ | assumption].
+      destruct H2 as [x [t H2]]; subst.
+      destruct (IHM2 M2 eq_refl JMeq_refl T2 H3); [ | destruct H0]; eauto.
+    + (* t1 can step *)
+      destruct H0. eauto.
+Qed.
